compiler/backend/languages/semantics/thunkLangScript.sml
@@ -180,6 +180,11 @@ Definition dest_anyThunk_def:
     od
 End
 
+Definition is_anyThunk_def:
+  is_anyThunk (DoTick v) = is_anyThunk v ∧
+  is_anyThunk v = ∃tv. dest_anyThunk v = INR tv
+End
+
 Definition dest_Constructor_def[simp]:
   dest_Constructor (Constructor s vs) = return (s, vs) ∧
   dest_Constructor _ = fail Type_error
@@ -284,7 +289,8 @@ Definition eval_to_def:
            SOME w => eval_to (k - 1) (Force (Value w))
          | NONE =>
              do (y, binds) <- dest_anyThunk v;
-                eval_to (k - 1) (subst_funs binds y)
+                res <- eval_to (k - 1) (subst_funs binds y);
+                if is_anyThunk res then fail Type_error else return res
              od
        od) ∧
   eval_to k (MkTick x) =
@@ -471,8 +477,8 @@ Proof
     \\ Cases_on ‘eval_to k x’ \\ fs []
     \\ BasicProvers.TOP_CASE_TAC \\ gs []
     \\ Cases_on ‘dest_anyThunk y’ \\ gs []
-    \\ pairarg_tac \\ gvs [])
-    (* \\ BasicProvers.TOP_CASE_TAC \\ gs []) *)
+    \\ pairarg_tac \\ gvs []
+    \\ Cases_on `eval_to (k - 1) (subst_funs binds y'')` \\ gvs [])
   >- ((* MkTick *)
     rw [eval_to_def]
     \\ Cases_on ‘eval_to k x’ \\ fs [])
